define and starting verifying a special compiler for the repl call
the problem is we want to run the code for calling repl_step multiple
times, so it should already be there in the bytecode machine at the
start, but the compiler's invariants are set up assuming you are about
to install the new code. this can all be worked around if we know the
code doesn't contain any labels, which should be true for the code for
calling repl_step, but the normal compiler has error handlers and other
things involving labels. so define a special compiler for code that is
known to terminate succesfully and not introduce any bindings and not
contain any functions (hence no labels), which skips the code
environment generation and the error handling.

compiler/proofs/compilerProofScript.sml
@@ -3939,4 +3939,303 @@ val compile_prog_divergence = store_thm("compile_prog_divergence",
   HINT_EXISTS_TAC >>
   simp[Abbr`bs0`])
 
+(* compile_special, for the repl *)
+
+val prompt_to_i3_special_def = Define`
+  prompt_to_i3_special none_tag next (Prompt_i2 ds) =
+    Let_i2 NONE (decs_to_i3 next ds) (Con_i2 none_tag [])`
+
+val prompt_to_i3_special_correct = store_thm("prompt_to_i3_special_correct",
+  ``∀ck (exh:exh_ctors_env) genv s p new_env s' next' e.
+    evaluate_prompt_i2 ck exh genv s (Prompt_i2 p) (s',new_env,NONE) ⇒
+    num_defs p = 0 ∧
+    (e = prompt_to_i3_special (none_tag,SOME(TypeId(Short"option"))) (LENGTH genv) (Prompt_i2 p)) ⇒
+    evaluate_i3 ck (exh,[]) (s,genv) e ((s',genv++new_env),Rval(Conv_i2 (none_tag,SOME(TypeId(Short"option")))[]))``,
+  simp[prompt_to_i3_special_def] >>
+  simp[evaluate_prompt_i2_cases,PULL_EXISTS] >>
+  rw[] >>
+  first_x_assum(mp_tac o MATCH_MP (REWRITE_RULE[GSYM AND_IMP_INTRO]decs_to_i3_correct)) >>
+  simp[dec_result_to_i3_cases,PULL_EXISTS] >> rw[] >>
+  simp[Once evaluate_i3_cases] >>
+  first_assum(match_exists_tac o concl) >> rw[] >>
+  simp[Once evaluate_i3_cases] >>
+  simp[Once evaluate_i3_cases])
+
+val free_vars_i2_prompt_to_i3_special = store_thm("free_vars_i2_prompt_to_i3_special",
+  ``∀x s p. free_vars_i2 (prompt_to_i3_special x s p) = free_vars_prompt_i2 p``,
+  Cases_on`p`>>simp[prompt_to_i3_special_def] >>
+  simp[free_vars_i2_decs_to_i3])
+
+val compile_special_def = Define`
+  compile_special cs top =
+    let n = cs.next_global in
+    let (m1,m2) = cs.globals_env in
+    let (v,m1,m2,p) = top_to_i1 n m1 m2 top in
+    let (c,exh,p) = prompt_to_i2 cs.contags_env p in
+    let e = prompt_to_i3_special (none_tag,SOME(TypeId(Short"option"))) n p in
+    let exh = exh ⊌ cs.exh in
+    let e = exp_to_exh exh e in
+    let e = exp_to_pat [] e in
+    let e = exp_to_Cexp e in
+    let r = compile [] TCNonTail 0 <|out:=[];next_label:=cs.rnext_label|> e in
+    (emit r [Stack Pop; Stop T]).out`
+
+val no_functions_def = tDefine"no_functions"`
+  (no_functions (Fun _ _) = F) ∧
+  (no_functions (Letrec _ _ ) = F) ∧
+  (no_functions (Raise e) = no_functions e) ∧
+  (no_functions (Handle _ pes) = EVERY no_functions (MAP SND pes)) ∧
+  (no_functions (Con _ es) = EVERY no_functions es) ∧
+  (no_functions (Uapp _ e) = no_functions e) ∧
+  (no_functions (App _ e1 e2) ⇔ no_functions e1 ∧ no_functions e2) ∧
+  (no_functions (Log _ e1 e2) ⇔ no_functions e1 ∧ no_functions e2) ∧
+  (no_functions (If e1 e2 e3) ⇔ no_functions e1 ∧ no_functions e2 ∧ no_functions e3) ∧
+  (no_functions (Mat e pes) ⇔ no_functions e ∧ EVERY no_functions (MAP SND pes)) ∧
+  (no_functions _ = T)`
+  (WF_REL_TAC`measure exp_size` >> simp[] >>
+   rpt conj_tac >> gen_tac >> Induct >>
+   simp[exp_size_def] >>
+   TRY (
+     rpt gen_tac >> strip_tac >> simp[] >>
+     res_tac >> simp[]>>NO_TAC) >>
+   Cases >> simp[exp_size_def] >>
+   rpt gen_tac >> strip_tac >> simp[] >>
+   res_tac >> simp[])
+
+val no_functions_dec_def = Define`
+  no_functions_dec (Dlet p e) = no_functions e ∧
+  no_functions_dec (Dletrec _) = F ∧
+  no_functions_dec _ = T`
+
+val no_functions_top_def = Define`
+  no_functions_top (Tdec dec) = no_functions_dec dec ∧
+  no_functions_top _ = F`
+
+(*
+val compile_special_thm = store_thm("compile_special_thm",
+  ``∀ck env stm top res. evaluate_top ck env stm top res ⇒
+     ∀rs grd bc bc0 bs s0 tm s.
+      env_rs env stm grd rs bs ∧
+      (compile_special rs top = bc) ∧
+      closed_top env top ∧
+      no_functions_top top ∧
+      FILTER is_Label bc = [] ∧
+      (bs.code = bc0 ++ REVERSE bc) ∧
+      (bs.pc = next_addr bs.inst_length bc0) ∧
+      ck ∧ IS_SOME bs.clock ∧
+      stm = (s0,tm) ∧
+      res = ((s,tm), ([],[]), Rval([],[]))
+      ⇒
+        ∃bs' grd'.
+        bc_next^* bs bs' ∧
+        bc_fetch bs' = SOME (Stop T) ∧
+        bs'.output = bs.output ∧
+        env_rs env (s,tm) grd' rs bs'``,
+  ho_match_mp_tac evaluate_top_ind >> simp[] >>
+  simp[compile_special_def] >>
+  rpt gen_tac >> strip_tac >>
+  rpt gen_tac >> strip_tac >>
+  `∃m1 m2. rs.globals_env = (m1,m2)` by simp[GSYM EXISTS_PROD] >> fs[] >>
+  qspecl_then[`m1`,`m2`,`Tdec d`]mp_tac top_to_i1_correct >>
+  fs[libTheory.emp_def] >>
+  rpt BasicProvers.VAR_EQ_TAC >> rpt(qpat_assum`T`kall_tac) >>
+  PairCases_on`grd`>>PairCases_on`env`>>PairCases_on`s1`>>fs[env_rs_def] >>
+  REWRITE_TAC[Once CONJ_COMM] >>
+  REWRITE_TAC[Once (GSYM CONJ_ASSOC)] >>
+  REWRITE_TAC[Once (GSYM AND_IMP_INTRO)] >>
+  disch_then(fn th => first_assum (mp_tac o MATCH_MP th)) >>
+  `∃v w z p1. top_to_i1 rs.next_global m1 m2 (Tdec d) = (v,w,z,p1)` by simp[GSYM EXISTS_PROD] >> fs[] >>
+  simp[Once evaluate_top_cases] >>
+  simp_tac(srw_ss()++DNF_ss)[] >>
+  disch_then(mp_tac o CONJUNCT1) >> rfs[] >>
+  disch_then(fn th => first_assum (mp_tac o MATCH_MP th)) >>
+  disch_then(qx_choosel_then[`s2_i1`,`new_genv`]strip_assume_tac) >>
+  `∃c exh p. prompt_to_i2 rs.contags_env p1 = (c,exh,p)` by simp[GSYM EXISTS_PROD] >> fs[] >>
+  first_assum (mp_tac o (MATCH_MP (
+    CONV_RULE (
+      ONCE_REWRITE_CONV[CONJ_ASSOC] THENC
+      ONCE_REWRITE_CONV[CONJ_COMM] THENC
+      ONCE_REWRITE_CONV[GSYM CONJ_ASSOC] THENC
+      ONCE_REWRITE_CONV[GSYM AND_IMP_INTRO]) prompt_to_i2_correct))) >>
+  REWRITE_TAC[Once EQ_SYM_EQ] >>
+  REWRITE_TAC[Once (GSYM CONJ_ASSOC)] >>
+  REWRITE_TAC[Once (GSYM AND_IMP_INTRO)] >>
+  disch_then(fn th => first_assum (mp_tac o MATCH_MP th)) >>
+  REWRITE_TAC[Once (GSYM AND_IMP_INTRO)] >>
+  disch_then(fn th => first_assum (mp_tac o MATCH_MP th)) >>
+  simp[] >>
+  disch_then(qx_choosel_then[`new_genv_i2`,`s2_i2`,`gtagenv2`]strip_assume_tac) >>
+  Cases_on`p` >>
+  first_x_assum(mp_tac o MATCH_MP prompt_to_i3_special_correct) >>
+  `new_dec_vs d = []` by (
+    imp_res_tac evaluate_dec_new_dec_vs >> fs[] ) >>
+  simp[] >>
+  discharge_hyps >- (
+    fs[top_to_i1_def,LET_THM] >>
+    first_assum(split_applied_pair_tac o lhs o concl) >> fs[] >>
+    imp_res_tac dec_to_i1_new_dec_vs >> rfs[] >> fs[LENGTH_NIL] >>
+    rpt BasicProvers.VAR_EQ_TAC >>
+    fs[Once evaluate_prompt_i1_cases] >>
+    fs[Once evaluate_decs_i1_cases] >>
+    fs[Once evaluate_decs_i1_cases] >>
+    fs[prompt_to_i2_def,LET_THM] >>
+    first_assum(split_applied_pair_tac o lhs o concl) >> fs[] >>
+    rpt BasicProvers.VAR_EQ_TAC >>
+    fs[decs_to_i2_def,LET_THM] >>
+    Cases_on`d`>>fs[dec_to_i1_def,LET_THM,LENGTH_NIL]>>rw[]>>fs[]>>rw[]>>
+    simp[num_defs_def,funs_to_i1_MAP,funs_to_i2_MAP] ) >>
+  strip_tac >>
+  first_assum (mp_tac o MATCH_MP (CONJUNCT1 exp_to_exh_correct)) >>
+  simp[env_to_exh_MAP,result_to_exh_cases,PULL_EXISTS,Once v_to_exh_cases,vs_to_exh_MAP] >>
+  fs[LIST_REL_O,OPTREL_O] >>
+  qmatch_assum_abbrev_tac`LIST_REL (v_to_exh rsexh) s20 sh` >>
+  qmatch_assum_rename_tac`LIST_REL R genv2 gh`["R"] >>
+  `store_to_exh (exh ⊌ rsexh) ((s10,s20),genv2) ((s10,sh),gh)` by (
+    simp[store_to_exh_def] >>
+    conj_tac >>
+    match_mp_tac (MP_CANON (GEN_ALL EVERY2_mono)) >>
+    HINT_EXISTS_TAC >>
+    metis_tac[optionTheory.OPTREL_MONO,v_to_exh_extend_disjoint,FUNION_COMM,DISJOINT_SYM]) >>
+  disch_then(fn th => first_assum (mp_tac o MATCH_MP (ONCE_REWRITE_RULE[GSYM AND_IMP_INTRO]th))) >>
+  disch_then(qspec_then`exh ⊌ rsexh`mp_tac) >> simp[] >>
+  strip_tac >>
+  (exp_to_pat_correct
+   |> CONJUNCT1
+   |> (fn th => first_assum (mp_tac o MATCH_MP th))) >>
+  simp[Once v_pat_cases] >>
+  strip_tac >>
+  first_assum (mp_tac o MATCH_MP (CONJUNCT1 exp_to_Cexp_correct)) >>
+  simp[] >>
+  discharge_hyps_keep >- (
+    conj_asm1_tac >- (
+      specl_args_of_then``exp_to_pat``(CONJUNCT1 free_vars_pat_exp_to_pat)mp_tac >>
+      simp[] >> disch_then match_mp_tac >>
+      simp[free_vars_i2_prompt_to_i3_special] >>
+      imp_res_tac free_vars_prompt_to_i2 >>
+      imp_res_tac FV_top_to_i1 >>
+      fs[closed_top_def,all_env_dom_def,SUBSET_DEF,PULL_EXISTS] >>
+      simp[EXTENSION] >> rw[] >>
+      CCONTR_TAC >> fs[] >> res_tac >> fs[] >> rw[] >>
+      fs[to_i1_invariant_def] >>
+      imp_res_tac global_env_inv_inclusion >>
+      fs[SUBSET_DEF]) >>
+    simp[csg_closed_pat_def,map_count_store_genv_def,store_to_exh_def] >>
+    conj_tac >- (
+      (v_to_pat_closed |> CONJUNCT2 |> SIMP_RULE(srw_ss())[] |> match_mp_tac) >>
+      (v_to_exh_closed |> CONJUNCT2 |> CONJUNCT1 |> MP_CANON |> match_mp_tac) >>
+      fs[store_to_exh_def] >>
+      simp[vs_to_exh_MAP] >>
+      first_assum(match_exists_tac o concl) >> simp[] >>
+      fs[to_i2_invariant_def] >>
+      fs[Once s_to_i2_cases] >>
+      fs[Once s_to_i2'_cases] >>
+      (v_to_i2_closed |> CONJUNCT2 |> CONJUNCT1 |> MP_CANON |> match_mp_tac) >>
+      first_assum(match_exists_tac o concl) >> simp[] >>
+      (v_to_i1_closed |> CONJUNCT2 |> CONJUNCT1 |> MP_CANON |> match_mp_tac) >>
+      fs[to_i1_invariant_def] >>
+      fs[Once s_to_i1_cases] >>
+      fs[Once s_to_i1'_cases] >>
+      first_assum(match_exists_tac o concl) >> simp[]) >>
+    match_mp_tac genv_to_pat_closed >>
+    match_mp_tac genv_to_exh_closed >>
+    fs[store_to_exh_def] >>
+    ONCE_REWRITE_TAC[CONJ_COMM] >>
+    first_assum(match_exists_tac o concl) >> simp[] >>
+    fs[to_i2_invariant_def] >>
+    match_mp_tac (MP_CANON genv_to_i2_closed) >>
+    first_assum(match_exists_tac o concl) >> simp[]>>
+    first_assum(match_exists_tac o concl) >> simp[]) >>
+  disch_then(qx_choosel_then[`Cres0`]strip_assume_tac) >>
+  first_assum(mp_tac o MATCH_MP (CONJUNCT1 Cevaluate_syneq)) >>
+  simp[] >>
+  Q.PAT_ABBREV_TAC`Cexp = exp_to_Cexp Z` >>
+  qmatch_assum_abbrev_tac`closed_vlabs [] Csg XX` >>
+  disch_then(qspecl_then[`$=`,`Csg`,`[]`,`Cexp`]mp_tac) >>
+  discharge_hyps >- (
+    simp[syneq_exp_refl] >>
+    fs[store_to_exh_def] >>
+    simp[Abbr`Csg`,map_count_store_genv_def,csg_rel_def] >>
+    simp[MAP_MAP_o,optionTheory.OPTION_MAP_COMPOSE,combinTheory.o_DEF] >>
+    simp[EVERY2_MAP] >>
+    conj_tac >>
+    match_mp_tac EVERY2_MEM_MONO >>
+    HINT_EXISTS_TAC >>
+    simp[exh_Cv_def,optionTheory.OPTREL_def,UNCURRY] >- (
+      rw[] >> rw[] >>
+      first_x_assum(mp_tac o MATCH_MP v_pat_syneq) >>
+      discharge_hyps >- (
+        simp[] >>
+        fs[csg_closed_pat_def,EVERY_MAP,EVERY_MEM] >>
+        first_x_assum match_mp_tac >>
+        simp[map_count_store_genv_def,MEM_MAP] >>
+        qexists_tac`FST x` >> simp[] >>
+        imp_res_tac MEM_ZIP_MEM_MAP >>
+        imp_res_tac EVERY2_LENGTH >> fs[] ) >>
+      metis_tac[syneq_trans] ) >>
+    rw[] >> rw[] >>
+    first_x_assum(mp_tac o MATCH_MP v_pat_syneq) >>
+    discharge_hyps >- (
+      simp[] >>
+      fs[csg_closed_pat_def,EVERY_MAP,EVERY_MEM] >>
+      first_x_assum(qspec_then`OPTION_MAP v_to_pat (FST x)`mp_tac) >>
+      simp[map_count_store_genv_def] >>
+      disch_then match_mp_tac >>
+      simp[MEM_MAP,PULL_EXISTS] >>
+      metis_tac[MEM_ZIP_MEM_MAP,EVERY2_LENGTH,FST,SND] ) >>
+    metis_tac[syneq_trans] ) >>
+  strip_tac >>
+  first_assum(mp_tac o MATCH_MP (CONJUNCT1 compile_val)) >>
+  simp[] >>
+  Cases_on`res2`>>fs[] >>
+  rator_x_assum`Cenv_bs`assume_tac >>
+  rator_x_assum`closed_vlabs`assume_tac >>
+  disch_then(qspecl_then[`grd2`,`<|out:=[];next_label:=rs.rnext_label|>`,`[]`,`0`,`bs`,`bs.code`]mp_tac) >>
+  qmatch_assum_abbrev_tac`Abbrev(XX=bc0++YY++ZZ)`>>
+  simp[Abbr`XX`] >>
+  disch_then(qspecl_then[`[]`,`bc0`]mp_tac) >> simp[] >>
+  `LENGTH genv2 = LENGTH grd0` by (
+    fs[to_i2_invariant_def] >>
+    imp_res_tac EVERY2_LENGTH >>
+    fs[] ) >>
+  fs[] >> rfs[] >>
+  disch_then(qspec_then`YY`mp_tac) >> simp[] >>
+  discharge_hyps >- (
+    fs[closed_vlabs_def] >>
+    rator_x_assum`good_labels`assume_tac >>
+    fs[good_labels_def,FILTER_APPEND,ALL_DISTINCT_APPEND,Abbr`YY`,Abbr`ZZ`] >>
+    conj_tac >- cheat >>
+    conj_tac >- cheat >>
+    fs[all_vlabs_csg_def,vlabs_csg_def] >>
+    conj_tac >- (
+      fs[Cenv_bs_def,s_refs_def] >>
+      metis_tac[IS_SOME_EXISTS] ) >>
+    qsuff_tac`set(free_vars Cexp) = {}`>-rw[]>>
+    qunabbrev_tac`Cexp` >>
+    REWRITE_TAC[Once free_vars_exp_to_Cexp] >>
+    simp[] ) >>
+  discharge_hyps >- simp[Abbr`YY`] >>
+  simp[code_for_push_def,PULL_EXISTS] >>
+  rpt gen_tac >> strip_tac >>
+  qmatch_assum_abbrev_tac`bc_next^* bs bs1` >>
+  `bc_fetch bs1 = SOME (Stack Pop)` by (
+    match_mp_tac bc_fetch_next_addr >>
+    simp[Abbr`bs1`] >>
+    qexists_tac`bc0++YY` >> simp[Abbr`ZZ`] ) >>
+  srw_tac[DNF_ss][Once RTC_CASES2] >> disj2_tac >>
+  first_assum(match_exists_tac o concl) >>
+  simp[bc_eval1_thm,bc_eval1_def] >>
+  simp[Abbr`bs1`,bc_eval_stack_def] >>
+  simp[RIGHT_EXISTS_AND_THM] >>
+  conj_tac >- (
+    match_mp_tac bc_fetch_next_addr >>
+    simp[bump_pc_def] >>
+    CONV_TAC SWAP_EXISTS_CONV >>
+    qexists_tac`[]`>>simp[Abbr`ZZ`] >>
+    simp[SUM_APPEND,FILTER_APPEND] ) >>
+  simp[bump_pc_def] >>
+  simp[EXISTS_PROD] >>
+  Cases_on`s2`>> simp[env_rs_def,PULL_EXISTS] >>
+  rator_x_assum`to_i1_invariant`assume_tac
+*)
+
 val _ = export_theory()
